theories/TM/L/CompilerBoolFuns/LComp_to_TMComp.v
@@ -1,9 +1,13 @@
 From Undecidability.TM.L.CompilerBoolFuns Require Import Compiler_spec Compiler_facts Compiler ClosedLAdmissible.
 
-Lemma L_computable_is_TM_computable k (R : Vector.t (list bool) k -> list bool -> Prop) :
+Lemma L_bool_computable_to_TM_bool_computable k (R : Vector.t (list bool) k -> list bool -> Prop) :
   L_bool_computable R -> TM_bool_computable R.
 Proof.
   intros H. eapply TM_bool_computable_hoare'_spec.
   -now apply L_bool_computable_function.
   -now eapply compiler_correct, L_bool_computable_can_closed.
 Qed.
+
+Lemma L_computable_to_TM_computable k (R : Vector.t nat k -> nat -> Prop) :
+  L_computable R -> TM_computable R.
+Admitted.
